src/Narcissus/Formats/Option.v
@@ -9,23 +9,46 @@ Unset Implicit Arguments.
 Section Option.
 
   Context {sz : nat}.
-  Context {A : Type}.
-  Context {B : Type}.
+  Context {S : Type}.
+  Context {T : Type}.
   Context {cache : Cache}.
   Context {cacheAddNat : CacheAdd cache nat}.
-  Context {monoid : Monoid B}.
+  Context {monoid : Monoid T}.
 
   Definition format_option
-             (format_Some : A -> CacheFormat -> Comp (B * CacheFormat))
-             (format_None : () -> CacheFormat -> Comp (B * CacheFormat))
-             (a_opt : option A)
-    := If_Opt_Then_Else a_opt format_Some (format_None ()).
+             (format_Some : FormatM S T)
+             (format_None : FormatM () T)
+    : FormatM (option S) T :=
+    fun a_opt => If_Opt_Then_Else a_opt format_Some (format_None ()).
+
+  Definition option_encode
+             (encode_Some : EncodeM S T)
+             (encode_None : EncodeM () T)
+    : EncodeM (option S) T :=
+    fun a_opt => If_Opt_Then_Else a_opt encode_Some (encode_None ()).
+
+  Definition option_decode
+             (decode_Some : DecodeM (S * T) T)
+             (decode_None : DecodeM (() * T) T)
+             (b' : bool)
+    : DecodeM ((option S) * T) T :=
+    (fun (b : T) (env : CacheDecode) =>
+       If b' Then
+          match decode_Some b env with
+          | Some (a, b, c) => Some ((Some a, b), c)
+          | None => None
+          end
+          Else
+          match decode_None b env with
+          | Some (a, b, c) => Some ((None, b), c)
+          | None => None
+          end).
 
   Lemma option_format_correct
       {P  : CacheDecode -> Prop}
       {P_invT P_invE : (CacheDecode -> Prop) -> Prop}
       (P_inv_pf : cache_inv_Property P (fun P => P_invT P /\ P_invE P))
-      (predicate_Some : A -> Prop)
+      (predicate_Some : S -> Prop)
       (predicate_None : () -> Prop)
       (b' : bool)
       (predicate :=
@@ -35,18 +58,18 @@ Section Option.
               | Some a => predicate_Some a
               | None => predicate_None ()
               end)
-      (predicate_rest_Some : A -> B -> Prop)
-      (predicate_rest_None : () -> B -> Prop)
+      (predicate_rest_Some : S -> T -> Prop)
+      (predicate_rest_None : () -> T -> Prop)
       (predicate_rest :=
          fun a_opt =>
            match a_opt with
            | Some a => predicate_rest_Some a
            | None => predicate_rest_None ()
            end)
-      (format_Some : A -> CacheFormat -> Comp (B * CacheFormat))
-      (decode_Some : B -> CacheDecode -> option (A * B * CacheDecode))
-      (format_None : () -> CacheFormat -> Comp (B * CacheFormat))
-      (decode_None : B -> CacheDecode -> option (() * B * CacheDecode))
+      (format_Some : FormatM S T)
+      (format_None : FormatM () T)
+      (decode_Some : DecodeM (S * T) T)
+      (decode_None : DecodeM (() * T) T)
       (decode_Some_pf :
          cache_inv_Property P P_invT
          -> CorrectDecoder
@@ -62,23 +85,13 @@ Section Option.
       predicate
       predicate_rest
       (format_option format_Some format_None)%comp
-      (fun (b : B) (env : CacheDecode) =>
-         If b' Then
-            match decode_Some b env with
-            | Some (a, b, c) => Some (Some a, b, c)
-            | None => None
-            end
-            Else
-            match decode_None b env with
-            | Some (a, b, c) => Some (None, b, c)
-            | None => None
-            end
-      ) P.
+      (option_decode decode_Some decode_None b')
+ P.
 Proof.
   unfold cache_inv_Property in *; split.
   { intros env env' xenv data bin ext ? env_pm pred_pm pred_pm_rest com_pf.
     unfold format_option in com_pf; computes_to_inv;
-      destruct data;
+      unfold option_decode; destruct data;
       find_if_inside; unfold predicate in *; simpl in *;
         intuition; try discriminate.
     - eapply H3 in com_pf; destruct_ex;
@@ -86,7 +99,7 @@ Proof.
     - eapply H4 in com_pf; destruct_ex;
         intuition eauto; rewrite H6; eauto.
   }
-  { intros.
+  { unfold option_decode; intros.
     find_if_inside; simpl in *.
     - destruct (decode_Some bin env') as [ [ [? ?] ?] | ] eqn : ? ;
         simpl in *; try discriminate; injections; simpl.
